feat: add MyImpl2.v

MyImpl2.v
@@ -1,4 +1,4 @@
-Set Warnings "-notation-overridden,-parsing".
+                                        Set Warnings "-notation-overridden,-parsing".
 From PLF Require Import Smallstep.
 From Coq Require Import Strings.String.
 
@@ -151,17 +151,24 @@ Inductive beta_equiv :tm -> tm -> Prop:=
   | beta_l t1 t1' t2: t1 =b t1' -> app t1 t2 =b app t1' t2
   | beta_r t1 t2 t2': t2 =b t2' -> app t1 t2 =b app t1 t2' 
   | beta_appabs x t h:
-                halt h ->
                 (app (abs x t) h) =b (subst x h t)
+  | beta_abs x t t':
+                t =b t' ->
+                abs x t =b abs x t'
   | beta_fix1 t1 t1': t1 =b t1' -> tfix t1 =b tfix t1'
   | beta_fixabs f t2: tfix (abs f t2) =b subst f (tfix (abs f t2)) t2 
-  | beta_test01: forall t1 t1' t2 t3,
+  | beta_test01: forall t1 t1' t2 t2' t3 t3',
               t1 =b t1' ->
-              (test0 t1 t2 t3) =b (test0 t1' t2 t3)
-  | beta_test0Zro t2 t3 : 
-              (test0 0 t2 t3) =b t2
-  | beta_test0NotZro n t2 t3: 
-              (test0 (S n) t2 t3) =b t3
+              t2 =b t2' ->
+              t3 =b t3' ->
+              (test0 t1 t2 t3) =b (test0 t1' t2' t3')
+  | beta_let1 : forall x t1 t2 t1' t2',
+              t1 =b t1' ->
+              t2 =b t2' ->
+              (tlet x t1 t2) =b (tlet x t1' t2')
+  | beta_letvalue : forall x h1 t2,
+              halt h1 ->
+              (tlet x h1 t2) =b (subst x h1 t2)
 where "t1 '=b' t2" := (beta_equiv t1 t2).
 Hint Constructors beta_equiv.
 
@@ -431,6 +438,62 @@ Definition sum_list_cont :=
               (abs "s" (Cont Nat) (app (var c) (pls (var hd) (var "s"))))))))).s
 **)
 
+Fixpoint l_have_string (l:list string) (k:string) : bool :=
+  match l with
+  | nil => false
+  | cons x l' => if eqb x k
+             then true
+             else l_have_string l' k
+  end.
+
+Fixpoint gen_sym_loop (l:list string) (k:string) (n:nat) (m:nat): string :=
+  match m with
+  | O => match n with
+        | O => k
+        | S n' => if(l_have_string l k) 
+                  then gen_sym_loop l (k++k) n' O
+                  else k
+        end
+  | S m' => match n with
+        | O => k
+        | S n' => if(l_have_string l k)
+                  then gen_sym_loop l (k++k) n' m
+                  else gen_sym_loop l (k++k) n' m'
+        end
+end.
+
+
+Definition gen_sym (l:list string) (m:nat): string :=
+  gen_sym_loop l "k" ((Datatypes.length l) + m) m.
+
+Fixpoint get_all_string (t:tm) : list string :=
+  match t with
+  | var y => y::nil
+  | app t1 t2 => (get_all_string t1) ++ (get_all_string t2)
+  | abs y t1 => y :: (get_all_string t1)
+  | nat_const n => nil
+  | op_const n => nil
+  | test0 t1 t2 t3 => (get_all_string t1) ++ (get_all_string t2) ++(get_all_string t3)
+  | tlet y t1 t2 => y::(get_all_string t1)++ (get_all_string t2)
+  | tfix t1 => get_all_string t1
+
+(*   | tnil T => false
+  | tcons t1 t2 => if (have_string x t1) 
+                    then true 
+                    else have_string x t2
+
+  | tlcase t1 t2 y1 y2 t3 => if (have_string x t1) 
+                              then true 
+                              else if (have_string x t2)
+                                  then true
+                                  else if eqb y1 x 
+                                      then false
+                                      else if eqb y2 x 
+                                        then false
+                                        else have_string x t3   *)
+end.
+
+
 Fixpoint have_string (x : string) (t:tm) :bool :=
   match t with
   | var y =>   
@@ -448,7 +511,7 @@ Fixpoint have_string (x : string) (t:tm) :bool :=
                       then true
                       else have_string x t3
   | tlet y t1 t2 => if eqb x y 
-                      then false
+                      then have_string x t1
                       else if (have_string x t1) 
                           then true 
                           else have_string x t2
@@ -481,7 +544,6 @@ Fixpoint has_app_F (t:tm) :bool :=
   | _ => false
 end.
 
-
 Fixpoint trans_M (F:string)(k t:tm) :=
   match (have_string F t) with
   | false => app k t
@@ -494,12 +556,12 @@ Fixpoint trans_M (F:string)(k t:tm) :=
             | app m1 m2 => if have_string F m1 
                   then if have_string F m2
                         then
-                          tlet "fs1"
-                            (abs "s1"  
-                              (tlet "fs2" 
-                                (abs "s2" (app k (app "s1" "s2")))
-                                (trans_M F "fs2" m2)))
-                            (trans_M F "fs1" m1)
+                          tlet "s1" 
+                            (abs "res1"
+                              (tlet "s2"
+                                (abs "res2" (app k (app "res1" "res2")))
+                                (trans_M F "s2" m2)))
+                            (trans_M F "s1" m1)
                         else
                             (trans_M F (abs "s" (app k (app "s" m2))) m1)
                   else if have_string F m2
@@ -510,6 +572,35 @@ Fixpoint trans_M (F:string)(k t:tm) :=
             | _ => app k t
             end
   end.
+
+(* Fixpoint trans_M (F:string)(k t:tm) (l:list string) :=
+  match (have_string F t) with
+  | false => app k t
+  | true => match t with 
+             (* F m => F' m k  *)
+            | app (var f) m => 
+                    if eqb f F
+                    then app (app F m) k
+                    else app k t
+            | app m1 m2 => if have_string F m1 
+                  then if have_string F m2
+                        then
+                          tlet (gen_sym l 1) 
+                            (abs (gen_sym l 2)  
+                              (tlet (gen_sym l 3)
+                                (abs (gen_sym l 4) (app k (app (gen_sym l 2) (gen_sym l 4))))
+                                (trans_M F (gen_sym l 3) m2 l)))
+                            (trans_M F (gen_sym l 1) m1 l)
+                        else
+                            (trans_M F (abs (gen_sym l 1) (app k (app (gen_sym l 1) m2))) m1 l)
+                  else if have_string F m2
+                        then
+                            (trans_M F (abs (gen_sym l 1) (app k (app m1 (gen_sym l 1))))  m2 l)
+                        else 
+                          app k t
+            | _ => app k t
+            end
+  end. *)
 (* Fixpoint trans_M (f : string) (k t3:tm) :=
   match t3 with 
   | app (var y) m => app t3 k
@@ -536,30 +627,28 @@ Fixpoint trans_M (F:string)(k t:tm) :=
   | _ => app t3 k
   end. *)
 
-Search (string).
-Print concat.
-Search list.
-
-
-Fixpoint l_have_string (l:list string) (k:string) : bool :=
-  match l with
-  | nil => false
-  | cons x l' => if eqb x k
-             then true
-             else l_have_string l' k
-  end.
-
-Fixpoint gen_sym_loop (l:list string) (k:string) (n:nat): string :=
-  match n with
-  | O => k
-  | S n' => if(l_have_string l k) 
-            then gen_sym_loop l (k++k) n'
-            else k
-  end.
-
-
-Definition gen_sym (l:list string): string :=
-  gen_sym_loop l "k" (Datatypes.length l).
+(* Definition trans_to_tail_recursion (F:tm):=
+  match F with
+  | tfix (abs f
+       (abs a t )) => match t with
+                        | test0 t1 t2 t3 => tfix (abs f
+                                              (abs a 
+                                                (abs (gen_sym (get_all_string F) 0)
+                                                  (test0 t1
+                                                    (app (gen_sym (get_all_string F) 0) t2)
+                                                    (trans_M f (gen_sym (get_all_string F) 0) t3 (get_all_string F))))))
+                    
+(*                         | tlcase t1 t2 y1 y2 t3 => tfix (abs f Tf
+                                                    (abs a Ta
+                                                      (abs k (Cont Ta)
+                                                        (tlcase t1 
+                                                          (app k t2)
+                                                          y1 y2
+                                                          (trans_M f k t3))))) *)
+                        | _ => F
+                        end
+  | _ => F
+  end. *)
 
 Definition trans_to_tail_recursion (F:tm):=
   match F with
@@ -567,10 +656,10 @@ Definition trans_to_tail_recursion (F:tm):=
        (abs a t )) => match t with
                         | test0 t1 t2 t3 => tfix (abs f
                                               (abs a 
-                                                (abs (gen_sym (cons a (cons f nil)))
+                                                (abs "k"
                                                   (test0 t1
-                                                    (app (gen_sym (cons a (cons f nil))) t2)
-                                                    (trans_M f (gen_sym (cons a (cons f nil))) t3)))))
+                                                    (app "k" t2)
+                                                    (trans_M f "k" t3 )))))
                     
 (*                         | tlcase t1 t2 y1 y2 t3 => tfix (abs f Tf
                                                     (abs a Ta
@@ -585,19 +674,18 @@ Definition trans_to_tail_recursion (F:tm):=
   end.
 
 
-
 Definition is_recursion (F:tm): Prop :=
   match F with
  | tfix (abs f 
-       (abs a t )) =>  if eqb f a 
+       (abs a t )) => if eqb f a 
                         then False
-                       else 
+                        else 
                         match t with
                         | test0 (var b) t2 t3 => if eqb a b
-                                                then if have_string f t2 
-                                                  then False
-                                                  else True
-                                                else False
+                                                  then if have_string f t2 
+                                                        then False
+                                                        else True
+                                                  else False
 (*                         | tlcase t1 t2 y1 y2 t3 => tfix (abs f Tf
                                                     (abs a Ta
                                                       (abs k (Cont Ta)
@@ -609,39 +697,27 @@ Definition is_recursion (F:tm): Prop :=
                         end
   | _ => False
   end.
-
-
-
-Check subst.
-
-Lemma subst_lemma1 : forall (F t: tm) (f:string), 
-  (have_string f F) = false -> subst f t F =b F.
-Proof.
-  intros.
-  unfold have_string in H.
-  induction t.
-  Admitted.
-
-Lemma subst_lemma2 : forall t1 t1' f s,
-  t1 =b t1' -> subst f s t1 =b subst f s t1'.
-Proof.
-  Admitted.
-
-Search list.
-
-Lemma gen_lemma : forall (x:string) (l:list string),
-  List.In x l -> x =? (gen_sym l) = false.
+(* Lemma gen_lemma : forall (x:string) (l:list string) (n:nat),
+  List.In x l -> x =? (gen_sym l n) = false.
 Proof.
   intros. 
   Admitted.
 
-Lemma gen_lemma2 : forall (l:list string),
-  (gen_sym l) =? (gen_sym l) = true.
+Lemma gen_lemma2 : forall (l:list string) (n:nat),
+  (gen_sym l n) =? (gen_sym l n) = true.
 Proof.
   intros.
   Search (_ =? _).
   apply eqb_refl.
   Qed.
+
+Lemma gen_lemma3 : forall (l:list string) (n m:nat),
+  n <> m ->
+  (gen_sym l n) =? (gen_sym l m) = false.
+Proof.
+  intros l.
+  Search (_ =? _).
+  Admitted. *)
 
 (* Lemma need_lemma1 : forall (x:string) (t:tm),
   t =b 
@@ -670,8 +746,6 @@ Proof.
   * eapply multi_step.
     apply H. eapply multi_refl.
   Qed.
-  
-Print beta_fixabs.
 
 Theorem multib_comm : forall (t1 t2:tm),
   multib t1 t2 -> multib t2 t1.
@@ -681,8 +755,459 @@ Proof.
   apply beta_symm. apply H.
   Qed.
 
+Fixpoint no_name_F (F : string) (M:tm) :Prop :=
+  match M with
+  | var y => True
+  | app t1 t2 => no_name_F F t1 /\ no_name_F F t2
+  | abs y t1 => 
+          if eqb y F then False else no_name_F F t1
+  | nat_const n => True
+  | op_const n => True
+  | test0 t1 t2 t3 => no_name_F F t1 /\ no_name_F F t2 /\ no_name_F F t3
+  | tlet y t1 t2 => if eqb F y 
+                      then False
+                      else no_name_F F t1 /\ no_name_F F t2
+  | tfix t1 => no_name_F F t1
+end.
 
-Theorem m_k : forall (F k:tm)(n: nat),
+Fixpoint match_subtm (f:string) (M:tm): Prop :=
+  match have_string f M with
+  | false => no_name_F f M
+  | true => match M with
+            | app m1 m2 => match m1 with
+                          | var a => if eqb f a
+                                    then if have_string f m2 
+                                      then False
+                                      else no_name_F f m2
+                                    else False
+                          | _ => match_subtm f m1 /\ match_subtm f m2
+                          end
+            | _ => False
+            end
+  end
+.
+
+Lemma subst_lemma1 : forall (f t: tm) (F:string), 
+  (have_string F f) = false -> subst F t f =b f.
+Proof.
+  intros.
+  induction f0.
+  - simpl. simpl in H. destruct (F =? s ) eqn:E1. 
+    + discriminate.
+    + apply beta_refl.
+  - simpl. apply multib_eq_be. eapply multi_step. apply beta_l. apply IHf0_1. simpl in H. destruct (have_string F f0_1) eqn:E1. discriminate. reflexivity.
+    eapply multi_step. apply beta_r. apply IHf0_2. simpl in H. destruct (have_string F f0_1) eqn:E1. discriminate. apply H.  apply multib_eq_be. apply beta_refl.
+  - simpl. simpl in H. destruct (F =? s) eqn:E1. apply beta_refl. apply beta_abs. apply IHf0. apply H.
+  - simpl. apply beta_refl.
+  - simpl. apply beta_refl.
+  - simpl. Print beta_equiv. simpl in H. destruct (have_string F f0_1) eqn:E1; destruct (have_string F f0_2) eqn:E2. apply beta_test01. apply IHf0_1. discriminate. discriminate. discriminate. discriminate. discriminate. apply beta_test01. apply IHf0_1. reflexivity. 
+    apply IHf0_2. reflexivity. apply IHf0_3. apply H.
+  - simpl. destruct (F =? s) eqn:E1. 
+    + apply beta_let1. apply IHf0_1. simpl in H. rewrite E1 in H. apply H. apply beta_refl.
+    + simpl in H. rewrite E1 in H. destruct (have_string F f0_1) eqn:E2. discriminate. apply beta_let1.  apply IHf0_1. reflexivity. apply IHf0_2. apply H.  
+  - simpl. Print beta_equiv. apply beta_fix1. apply IHf0. simpl in H. apply H.
+  Qed.
+
+Lemma subst_lemma2 : forall t1 t1' f s,
+  t1 =b t1' -> subst f s t1 =b subst f s t1'.
+Proof.
+  Admitted.
+
+Lemma subst_lemma3:forall t1 f s1 s1',
+  s1 =b s1' -> subst f s1 t1 =b subst f s1' t1.
+Proof.
+  Admitted.
+
+Lemma beta_rl : forall t1 t1' t2 t2',
+  t1 =b t1' ->
+  t2 =b t2' ->
+  app t1 t2 =b app t1' t2'.
+Proof.
+  intros.
+  apply multib_eq_be.
+  eapply multi_step.
+  - apply beta_l. apply H.
+  - eapply multi_step. apply beta_r. apply H0.
+  apply multib_eq_be.
+  apply beta_refl.
+  Qed.
+
+Lemma subst_lemma4:forall (f1 f2 :string) (t1 t2 t3:tm),
+  eqb f1 f2 = false->
+  have_string f2 t1 = false->
+  (*no_name_F f1 t3 ->*)
+  subst f1 t1 (subst f2 t2 t3) =b subst f2 (subst f1 t1 t2) (subst f1 t1 t3).
+Proof.
+  Admitted.
+(*   intros.
+  induction t3.
+  - simpl. destruct (f2 =? s) eqn:E1; destruct (f1 =? s) eqn:E2.
+    + apply eqb_eq in E1. apply eqb_eq in E2. subst. apply eqb_neq in H. destruct H. reflexivity.
+    + simpl. rewrite E1. apply beta_refl. 
+    + simpl. rewrite E2. apply beta_symm. apply subst_lemma1. apply H0.
+    + simpl. rewrite E1. rewrite E2. apply beta_refl.
+  - simpl. apply beta_rl.
+    + apply IHt3_1. simpl in H1. destruct H1. apply H1.
+    + apply IHt3_2. simpl in H1. destruct H1. apply H2. 
+  - simpl. destruct (f2 =? s) eqn:E1; destruct (f1 =? s) eqn:E2; simpl; try rewrite E1; try rewrite E2; try apply beta_refl.
+    + simpl in H1. apply eqb_eq in E2. rewrite E2 in H1. rewrite eqb_refl in H1. destruct H1.
+    + apply beta_abs. apply IHt3. simpl in H1. Search(_=?_). rewrite eqb_sym in E2. rewrite E2 in H1. apply H1. 
+  - simpl. apply beta_refl.
+  - simpl. apply beta_refl.
+  - simpl in H1. destruct H1. destruct H2. simpl. apply beta_test01. apply IHt3_1. apply H1.  apply IHt3_2. apply H2. apply IHt3_3. apply H3.
+  - simpl. destruct (f1 =? s) eqn:E2. 
+    + apply eqb_eq in E2. subst. simpl in H1. rewrite eqb_refl in H1. destruct H1.  
+    + destruct (f2 =? s) eqn:E1; simpl; try rewrite E1; try rewrite E2; try apply beta_refl.
+      * apply beta_let1. apply IHt3_1. simpl in H1. rewrite E2 in H1. destruct H1. apply H1. apply beta_refl.
+      * apply beta_let1. apply IHt3_1. simpl in H1. rewrite E2 in H1. destruct H1. apply H1. apply IHt3_2. simpl in H1. rewrite E2 in H1. destruct H1. apply H2.  
+  - simpl. Print beta_equiv. apply beta_fix1. apply IHt3. simpl in H1. apply H1.
+  Qed. *)
+
+
+
+
+Lemma match_subtm__no_name:forall (F:string) (M:tm),
+  match_subtm F M -> no_name_F F M.
+Proof.
+  intros.
+  induction M.
+  - simpl. reflexivity.
+  - simpl. simpl in H. destruct (have_string F M1) eqn:E1; destruct (have_string F M2) eqn:E2; split.
+    + apply IHM1. destruct M1 eqn:E3;try destruct H;try apply H.
+      * destruct (F=?s). destruct H. destruct H.
+    + apply IHM2. destruct M1 eqn:E3;try destruct H;try apply H0.
+      * destruct (F=?s). destruct H. destruct H.
+    + destruct M1 eqn:E3.
+      * simpl. reflexivity.
+      * apply IHM1. destruct H. apply H.
+      * apply IHM1. destruct H. apply H.
+      * apply IHM1. destruct H. apply H.
+      * apply IHM1. destruct H. apply H.
+      * apply IHM1. destruct H. apply H.
+      * apply IHM1. destruct H. apply H.
+      * apply IHM1. destruct H. apply H.
+    + destruct M1 eqn:E3.
+      * destruct (F=?s). apply H. destruct H.
+      * destruct H. apply IHM2. apply H0.
+      * destruct H. apply IHM2. apply H0.
+      * destruct H. apply IHM2. apply H0.
+      * destruct H. apply IHM2. apply H0.
+      * destruct H. apply IHM2. apply H0.
+      * destruct H. apply IHM2. apply H0.
+      * destruct H. apply IHM2. apply H0.
+    + apply IHM1. destruct M1 eqn:E3;try destruct H;try apply H.
+      * destruct (F=?s). destruct H. destruct H.
+    + apply IHM2. destruct M1 eqn:E3;try destruct H;try apply H0.
+      * destruct (F=?s). destruct H. destruct H.
+    + destruct H. apply H.
+    + destruct H. apply H0.
+  - simpl in H. destruct (F=?s) eqn:E1. 
+    + rewrite eqb_sym in H. rewrite E1 in H. destruct H.
+    + simpl. rewrite eqb_sym. rewrite E1. destruct (have_string F M). destruct H. rewrite eqb_sym in H. rewrite  E1 in H. apply H.
+  - simpl. reflexivity.
+  - simpl. reflexivity.
+  - simpl. simpl in H. 
+    destruct (have_string F M1). destruct H.
+    destruct (have_string F M2). destruct H.
+    destruct (have_string F M3). destruct H.
+    apply H.
+  - simpl. simpl in H. destruct (F=?s).
+    + destruct (have_string F M1). destruct H.
+      destruct (have_string F M2). destruct H.
+      destruct H.
+    + destruct (have_string F M1). destruct H.
+      destruct (have_string F M2). destruct H.
+      apply H.
+  - simpl. simpl in H. destruct (have_string F M). destruct H. apply H.
+  Qed. 
+Lemma subst_lemma5:forall (f1 f2:string) (t1 t2:tm),
+  eqb f1 f2 = false ->
+  have_string f1 t1 = false->
+  have_string f1 t2 = false->
+  have_string f1 (subst f2 t1 t2) = false.
+Proof.
+  intros.
+  induction t2.
+  - simpl. destruct (f2 =? s). apply H0. apply H1.
+  - simpl in H1. destruct (have_string f1 t2_1) eqn:E1. discriminate. apply IHt2_2 in H1. 
+    simpl. rewrite H1. assert(HH1: false = false). {reflexivity. } apply IHt2_1 in HH1. rewrite HH1. reflexivity.
+  - simpl. destruct (f2 =? s) eqn:E1. apply H1. simpl. destruct (f1=?s)eqn:E2. reflexivity. apply IHt2. simpl in H1. rewrite E2 in H1. apply H1.
+  - simpl. reflexivity.
+  - simpl. reflexivity.
+  - simpl. simpl in H1. destruct (have_string f1 t2_1) eqn:E1. discriminate. destruct (have_string f1 t2_2) eqn:E2. destruct H1. assert (HH1: true = true). { reflexivity. }
+    apply IHt2_1 in HH1. rewrite HH1. reflexivity.  assert (HH1: false = false). { reflexivity. } apply IHt2_1 in HH1. rewrite HH1. 
+    assert (HH2: false = false). { reflexivity. } apply IHt2_2 in HH2. rewrite HH2. apply IHt2_3. apply H1.
+  - simpl. destruct (f1 =? s) eqn:E1. apply IHt2_1. simpl in H1. rewrite E1 in H1. apply H1. 
+    simpl in H1. rewrite E1 in H1. destruct (have_string f1 t2_1) eqn:E2. discriminate. assert (HH1: false = false). { reflexivity. }  apply IHt2_1 in HH1.
+    rewrite HH1. destruct (f2 =? s). apply H1. apply IHt2_2. apply H1.
+  - simpl. apply IHt2. simpl in H1. apply H1.
+  Qed.
+Theorem m_k_2 : forall (f f' M k m:tm)(F:string),
+  have_string F k = false ->
+  match_subtm F M ->
+  eqb F "f" = true ->
+  (forall k' m',
+  app k' (app f m') =b app (app f' m') k') ->
+  have_string "s1" f' = false->
+  have_string "s2" f' = false->
+  have_string "s1" M = false->
+  have_string "s2" M = false ->
+  have_string "s2" f = false->
+  have_string "res1" f' = false->
+  have_string "res2" f' = false->
+  have_string "s1" f = false->
+  have_string "res1" f = false->
+  have_string "res2" f = false->
+  have_string "s" k = false->
+  have_string "s" f = false->
+  have_string "s" M = false->
+  have_string "s" f' = false->
+  have_string "res1" k = false->
+  have_string "res2" k = false->
+  have_string "res1" M = false->
+  have_string "res2" M = false->
+  subst F f' (trans_M F k M ) =b app k (subst F f M).
+
+Proof.
+  intros. 
+  apply multib_eq_be.
+  generalize dependent k0.
+  induction M;  intros.
+  - simpl. destruct (F =? s) eqn:E1.
+    + unfold match_subtm in H0. simpl in H0. rewrite E1 in H0. destruct H0. 
+    + simpl. rewrite E1. apply (subst_lemma1 k0 f' F) in H. eapply multi_step.
+      * apply beta_l. apply H.
+      * apply multib_eq_be. apply beta_refl.
+  -  destruct (have_string F M1) eqn:E1; destruct (have_string F M2) eqn:E2.
+    + destruct M1 as [] eqn:E4.
+      * destruct (s =? F) eqn:E3.
+        ** apply eqb_eq in E3. subst. simpl in H0. rewrite eqb_refl in H0. rewrite E2 in H0. destruct H0.
+        ** simpl. Search(_ =? _). simpl in E1. rewrite eqb_sym in E1. rewrite E3 in E1. discriminate.
+      * rewrite <- E4. apply eqb_eq in H1. eapply multi_step. rewrite <- E4 in E1.
+        ** apply subst_lemma2. simpl. rewrite E1. rewrite E4. rewrite E2. apply beta_letvalue. apply h_abs.
+        ** eapply multi_step.
+          *** apply subst_lemma2. apply subst_lemma3. apply beta_abs. apply beta_letvalue. apply h_abs.
+          *** eapply multi_step.
+            **** apply subst_lemma4. rewrite H1. simpl. reflexivity. apply H3. 
+            **** rewrite H1. simpl. eapply multi_step. 
+              ***** apply subst_lemma3. apply beta_abs. apply subst_lemma4. simpl. reflexivity. apply H4. 
+              ***** simpl. assert(HH1: (subst "f" f' (trans_M "f" "s2" M2)) =b (app "s2" (subst "f" f0 M2))).
+                   {apply multib_eq_be. rewrite H1 in IHM2. apply IHM2. - rewrite <- E4 in H0.  simpl in H0. rewrite <- E4 in E1. rewrite E1 in H0. rewrite E4 in H0. destruct H0. rewrite H1 in H21. apply H21. - rewrite <- E4 in H5. simpl in H5. destruct (have_string "s1" M1) eqn:EE1. discriminate H5. apply H5. 
+                  - rewrite <- E4 in H6. simpl in H6. destruct (have_string "s2" M1). discriminate. apply H6. 
+                  - rewrite <- E4 in H15. simpl in H15. destruct (have_string "s" M2) eqn:EE1. destruct (have_string "s" M1). discriminate H15. discriminate H15. reflexivity. 
+                  - rewrite <- E4 in H19. simpl in H19. destruct (have_string "res1" M1) eqn:EE1. discriminate. apply H19.
+                  - rewrite <- E4 in H20. simpl in H20. destruct (have_string "res2" M1) eqn:EE1. discriminate. apply H20.
+                  - simpl. reflexivity. -simpl. reflexivity. - simpl. reflexivity. - simpl. reflexivity. } 
+                  eapply multi_step.
+                  ++ apply subst_lemma3. apply beta_abs. apply subst_lemma2. apply HH1. 
+                  ++ simpl. eapply multi_step.
+                    +++ apply subst_lemma3. apply beta_abs. apply beta_r. apply subst_lemma1. apply subst_lemma5. simpl. reflexivity. apply H7. rewrite <- E4 in H6. simpl in H6. destruct (have_string "s2" M1) eqn:EE1. discriminate. apply H6.
+                    +++ eapply multi_step.
+                      ++++ apply subst_lemma3. apply beta_abs. apply beta_appabs.
+                      ++++ simpl. eapply multi_step.
+                        +++++ apply subst_lemma3. apply beta_abs. apply beta_l. apply subst_lemma1. apply subst_lemma5. simpl. reflexivity. apply H9. apply H18.
+                        +++++ assert(HH2: (subst "f" f' (trans_M "f" "s1" M1)) =b (app "s1" (subst "f" f0 M1))).
+                            { apply multib_eq_be. rewrite H1 in IHM1. rewrite <- E4 in IHM1. apply IHM1. 
+                              - rewrite <- E4 in H0.  simpl in H0. rewrite <- E4 in E1. rewrite E1 in H0. rewrite E4 in H0. destruct H0. rewrite <-E4 in H0. rewrite H1 in H0. apply H0. - rewrite <- E4 in H5. simpl in H5. destruct (have_string "s1" M1) eqn:EE1. discriminate H5. reflexivity. - rewrite <- E4 in H6. simpl in H6. destruct (have_string "s2" M1). discriminate H6. reflexivity.  - rewrite <-E4 in H15. simpl in H15. destruct (have_string "s" M1). discriminate. reflexivity. 
+                              - rewrite <- E4 in H19. simpl in H19. destruct (have_string "res1" M1) eqn:EE1. discriminate. reflexivity. 
+                              - rewrite <- E4 in H20. simpl in H20. destruct (have_string "res2" M1) eqn:EE1. discriminate. reflexivity.
+                              - simpl. reflexivity. - simpl. reflexivity. - simpl. reflexivity. - simpl. reflexivity. }  
+                            eapply multi_step.
+                          ++++++ apply subst_lemma2. apply HH2. 
+                          ++++++ simpl.  eapply multi_step.
+                            -- apply beta_appabs.
+                            -- simpl. eapply multi_step. apply beta_l. apply subst_lemma1. apply subst_lemma5. simpl. reflexivity. apply H8. apply H17.
+                               eapply multi_step. apply beta_r. apply beta_r. apply subst_lemma1. apply subst_lemma5. 
+                               simpl. reflexivity. apply H11. 
+                               rewrite <- E4 in H19. simpl in H19. destruct (have_string "res1" M1) eqn:EE1. discriminate. apply H19.
+                               eapply multi_step. apply beta_r. apply beta_l. apply subst_lemma1. apply subst_lemma5. simpl. reflexivity. apply H10.
+                               rewrite <- E4 in H5. simpl in H5. destruct (have_string "s1" M1) eqn:EE1. discriminate. reflexivity.
+                               eapply multi_step. apply beta_l. apply subst_lemma1. rewrite <- H1. apply H. apply multib_eq_be. apply beta_refl.
+      * rewrite <- E4 in H0; simpl in H0.  rewrite E2 in H0. rewrite <- E4 in E1. rewrite E1 in H0. rewrite E4 in H0. rewrite <- E4 in H0. 
+          destruct H0. rewrite E4 in H0. simpl in H0. 
+          rewrite E4 in E1. simpl in E1. rewrite E1 in H0. destruct H0.
+      * simpl in E1. discriminate E1.
+      * simpl in E1. discriminate E1.
+      * rewrite <- E4 in H0; simpl in H0.  rewrite E2 in H0. rewrite <- E4 in E1. rewrite E1 in H0. rewrite E4 in H0. rewrite <- E4 in H0. 
+          destruct H0. rewrite E4 in H0. simpl in H0. rewrite E4 in E1. simpl in E1. rewrite E1 in H0. destruct H0.
+      * rewrite <- E4 in H0; simpl in H0.  rewrite E2 in H0. rewrite <- E4 in E1. rewrite E1 in H0. rewrite E4 in H0. rewrite <- E4 in H0. 
+          destruct H0. rewrite E4 in H0. simpl in H0. rewrite E4 in E1. simpl in E1. rewrite E1 in H0. destruct H0.
+      * rewrite <- E4 in H0; simpl in H0.  rewrite E2 in H0. rewrite <- E4 in E1. rewrite E1 in H0. rewrite E4 in H0. rewrite <- E4 in H0. 
+          destruct H0. rewrite E4 in H0. simpl in H0. rewrite E4 in E1. simpl in E1. rewrite E1 in H0. destruct H0. 
+    + destruct M1 as [] eqn:E4.
+      * destruct (F =? s) eqn:E5. 
+        ** simpl. rewrite E5. Search(_ =? _). rewrite eqb_sym. rewrite E5. simpl. rewrite eqb_refl. eapply multi_step.
+          apply beta_l. apply beta_r. apply subst_lemma1. apply E2. eapply multi_step.
+          apply beta_r. apply subst_lemma1. apply H. apply multib_eq_be. apply beta_symm. apply multib_eq_be. eapply multi_step.
+          apply beta_r. apply beta_r. apply subst_lemma1. apply E2. apply multib_eq_be. apply H2.
+        ** simpl in E1. rewrite E5 in E1. discriminate E1.
+      * rewrite <- E4. rewrite <-E4 in E1. simpl. rewrite E1. rewrite E2. rewrite E4. eapply multi_step. apply multib_eq_be. apply IHM1. 
+        rewrite <-E4 in H0. simpl in H0. rewrite E1 in H0. rewrite E4 in H0. destruct H0. apply H0. rewrite <- E4 in H5. simpl in H5. 
+        ** destruct (have_string "s1" M1) eqn: EE1. 
+          *** discriminate.
+          *** rewrite <-E4. apply EE1.
+        ** destruct (have_string "s2" M1) eqn: EE2.
+          *** rewrite <- E4 in H6. simpl in H6. rewrite EE2 in H6. discriminate.
+          *** rewrite <- E4. apply EE2.
+        ** rewrite <- E4. rewrite <- E4 in H15. simpl in H15. destruct (have_string "s" M1) eqn:EE1. discriminate. reflexivity.
+        ** rewrite <- E4 in H19. simpl in H19. destruct (have_string "res1" M1) eqn:EE1. discriminate. rewrite <- E4. apply EE1. 
+        ** rewrite <- E4 in H20. simpl in H20. destruct (have_string "res2" M1) eqn:EE1. discriminate. rewrite <- E4. apply EE1. 
+        ** simpl. apply eqb_eq in H1. rewrite H1. simpl. rewrite <- H1. rewrite H. rewrite E2. reflexivity.  
+        ** simpl. reflexivity.
+        ** simpl. rewrite H17. rewrite <- E4 in H19. simpl in H19. destruct (have_string "res1" M1) eqn:EE1. discriminate. apply H19.
+        ** simpl. rewrite H18. rewrite <- E4 in H20. simpl in H20. destruct (have_string "res2" M1) eqn:EE1. discriminate. apply H20.
+        ** rewrite <- E4. eapply multi_step.
+           apply beta_appabs. simpl. eapply multi_step.
+           apply beta_l. apply subst_lemma1. apply H13. eapply multi_step.
+           apply beta_r. apply beta_r. apply subst_lemma1. rewrite <- E4 in H15. simpl in H15. destruct (have_string "s" M1) eqn:EE1. discriminate. apply H15. apply multib_eq_be.
+           apply beta_symm. apply multib_eq_be. eapply multi_step.
+           apply beta_r. apply beta_r. apply subst_lemma1. apply E2. apply multib_eq_be. apply beta_refl.
+      * rewrite <- E4 in H0; simpl in H0.  rewrite E2 in H0. rewrite <- E4 in E1. rewrite E1 in H0. rewrite E4 in H0. rewrite <- E4 in H0. 
+          destruct H0. rewrite E4 in H0. simpl in H0. rewrite E4 in E1. simpl in E1. rewrite E1 in H0. destruct H0.
+      * simpl in E1. discriminate.
+      * simpl in E1. discriminate.
+      * rewrite <- E4 in H0; simpl in H0.  rewrite E2 in H0. rewrite <- E4 in E1. rewrite E1 in H0. rewrite E4 in H0. rewrite <- E4 in H0. 
+          destruct H0. rewrite E4 in H0. simpl in H0. rewrite E4 in E1. simpl in E1. rewrite E1 in H0. destruct H0.
+      * rewrite <- E4 in H0; simpl in H0.  rewrite E2 in H0. rewrite <- E4 in E1. rewrite E1 in H0. rewrite E4 in H0. rewrite <- E4 in H0. 
+          destruct H0. rewrite E4 in H0. simpl in H0. rewrite E4 in E1. simpl in E1. rewrite E1 in H0. destruct H0. 
+      * rewrite <- E4 in H0; simpl in H0.  rewrite E2 in H0. rewrite <- E4 in E1. rewrite E1 in H0. rewrite E4 in H0. rewrite <- E4 in H0. 
+          destruct H0. rewrite E4 in H0. simpl in H0. rewrite E4 in E1. simpl in E1. rewrite E1 in H0. destruct H0. 
+    + simpl. rewrite E1. rewrite E2.
+      destruct M1 as [] eqn:E4.
+      * simpl in E1. destruct (F =? s) eqn:E5.
+        ** discriminate.
+        ** simpl in H0. rewrite E5 in H0. rewrite E2 in H0. destruct H0.
+      * eapply multi_step. apply multib_eq_be. apply IHM2. 
+        ** rewrite <-E4 in H0. simpl in H0. rewrite <- E4 in E1. rewrite E1 in H0. rewrite E2 in H0. rewrite E4 in H0. destruct H0. apply H21.
+        ** rewrite <- E4 in H5. simpl in H5. destruct (have_string "s1" M1) eqn:EE1. discriminate. apply H5.
+        ** rewrite <- E4 in H6. simpl in H6. destruct (have_string "s2" M1) eqn:EE1. discriminate. apply H6.
+        ** rewrite <- E4 in H15. simpl in H15. destruct (have_string "s" M1) eqn:EE1. discriminate. apply H15.
+        ** rewrite <- E4 in H19. simpl in H19. destruct (have_string "res1" M1) eqn:EE1. discriminate. apply H19. 
+        ** rewrite <- E4 in H20. simpl in H20. destruct (have_string "res2" M1) eqn:EE1. discriminate. apply H20.
+        ** simpl. apply eqb_eq in H1. rewrite H1. simpl. rewrite <- H1. rewrite H. simpl in E1. rewrite E1. reflexivity.
+        ** simpl. reflexivity.
+        ** rewrite <- E4. simpl. rewrite H17. rewrite <- E4 in H19. simpl in H19. destruct (have_string "res1" M1) eqn:EE1. discriminate. reflexivity. 
+        ** rewrite <- E4. simpl. rewrite H18. rewrite <- E4 in H20. simpl in H20. destruct (have_string "res2" M1) eqn:EE1. discriminate. reflexivity. 
+        ** rewrite <- E4. eapply multi_step. apply beta_appabs. eapply multi_step. simpl. apply beta_l. apply subst_lemma1. apply H13. eapply multi_step.
+           apply beta_r. apply beta_l. apply subst_lemma1. rewrite <-E4 in H15. simpl in H15. destruct (have_string "s" M1). discriminate. reflexivity.
+           apply multib_eq_be. apply beta_symm. apply multib_eq_be. eapply multi_step. apply beta_r. apply beta_l. apply subst_lemma1. rewrite E4. apply E1.
+           apply multib_eq_be. apply beta_refl.
+      * eapply multi_step. apply multib_eq_be. apply IHM2. 
+        ** rewrite <- E4 in H0. simpl in H0. rewrite <- E4 in E1. rewrite E1 in H0. rewrite E2 in H0. rewrite E4 in H0. destruct H0. apply H21.
+        ** rewrite <- E4 in H5. simpl in H5. destruct (have_string "s1" M1) eqn:EE1. discriminate. apply H5.
+        ** rewrite <- E4 in H6. simpl in H6. destruct (have_string "s2" M1) eqn:EE1. discriminate. apply H6.
+        ** rewrite <- E4 in H15. simpl in H15. destruct (have_string "s" M1) eqn:EE1. discriminate. apply H15.
+        ** rewrite <- E4 in H19. simpl in H19. destruct (have_string "res1" M1) eqn:EE1. discriminate. apply H19. 
+        ** rewrite <- E4 in H20. simpl in H20. destruct (have_string "res2" M1) eqn:EE1. discriminate. apply H20.
+        ** rewrite <- E4 in E1. rewrite <- E4. simpl. apply eqb_eq in H1. rewrite H1. simpl. rewrite <- H1. rewrite H.  simpl in E1. rewrite E1. reflexivity.
+        ** simpl. reflexivity.
+        ** rewrite <- E4. simpl. rewrite H17. rewrite <- E4 in H19. simpl in H19. destruct (have_string "res1" M1) eqn:EE1. discriminate. reflexivity. 
+        ** rewrite <- E4. simpl. rewrite H18. rewrite <- E4 in H20. simpl in H20. destruct (have_string "res2" M1) eqn:EE1. discriminate. reflexivity. 
+        ** rewrite <- E4. eapply multi_step. apply beta_appabs. eapply multi_step. simpl. apply beta_l. apply subst_lemma1. apply H13. eapply multi_step.
+           apply beta_r. apply beta_l. apply subst_lemma1. rewrite <-E4 in H15. simpl in H15. destruct (have_string "s" M1). discriminate. reflexivity.
+           apply multib_eq_be. apply beta_symm. apply multib_eq_be. eapply multi_step. apply beta_r. apply beta_l. apply subst_lemma1. rewrite E4. apply E1.
+           apply multib_eq_be. apply beta_refl.
+      * eapply multi_step. apply multib_eq_be. apply IHM2. 
+        ** rewrite <- E4 in H0. simpl in H0. rewrite <- E4 in E1. rewrite E1 in H0. rewrite E2 in H0. rewrite E4 in H0. destruct H0. apply H21.
+        ** rewrite <- E4 in H5. simpl in H5. destruct (have_string "s1" M1) eqn:EE1. discriminate. apply H5.
+        ** rewrite <- E4 in H6. simpl in H6. destruct (have_string "s2" M1) eqn:EE1. discriminate. apply H6.
+        ** rewrite <- E4 in H15. simpl in H15. destruct (have_string "s" M1) eqn:EE1. discriminate. apply H15.
+        ** rewrite <- E4 in H19. simpl in H19. destruct (have_string "res1" M1) eqn:EE1. discriminate. apply H19. 
+        ** rewrite <- E4 in H20. simpl in H20. destruct (have_string "res2" M1) eqn:EE1. discriminate. apply H20.
+        ** rewrite <- E4 in E1. rewrite <- E4. simpl. apply eqb_eq in H1. rewrite H1. simpl. rewrite <- H1. rewrite H.  simpl in E1. rewrite E1. reflexivity.
+        ** simpl. reflexivity.
+        ** rewrite <- E4. simpl. rewrite H17. rewrite <- E4 in H19. simpl in H19. destruct (have_string "res1" M1) eqn:EE1. discriminate. reflexivity. 
+        ** rewrite <- E4. simpl. rewrite H18. rewrite <- E4 in H20. simpl in H20. destruct (have_string "res2" M1) eqn:EE1. discriminate. reflexivity. 
+        ** rewrite <- E4. eapply multi_step. apply beta_appabs. eapply multi_step. simpl. apply beta_l. apply subst_lemma1. apply H13. eapply multi_step.
+           apply beta_r. apply beta_l. apply subst_lemma1. rewrite <-E4 in H15. simpl in H15. destruct (have_string "s" M1). discriminate. reflexivity.
+           apply multib_eq_be. apply beta_symm. apply multib_eq_be. eapply multi_step. apply beta_r. apply beta_l. apply subst_lemma1. rewrite E4. apply E1.
+           apply multib_eq_be. apply beta_refl.
+     * eapply multi_step. apply multib_eq_be. apply IHM2. 
+        ** rewrite <- E4 in H0. simpl in H0. rewrite <- E4 in E1. rewrite E1 in H0. rewrite E2 in H0. rewrite E4 in H0. destruct H0. apply H21.
+        ** rewrite <- E4 in H5. simpl in H5. destruct (have_string "s1" M1) eqn:EE1. discriminate. apply H5.
+        ** rewrite <- E4 in H6. simpl in H6. destruct (have_string "s2" M1) eqn:EE1. discriminate. apply H6.
+        ** rewrite <- E4 in H15. simpl in H15. destruct (have_string "s" M1) eqn:EE1. discriminate. apply H15.
+        ** rewrite <- E4 in H19. simpl in H19. destruct (have_string "res1" M1) eqn:EE1. discriminate. apply H19. 
+        ** rewrite <- E4 in H20. simpl in H20. destruct (have_string "res2" M1) eqn:EE1. discriminate. apply H20.
+        ** rewrite <- E4 in E1. rewrite <- E4. simpl. apply eqb_eq in H1. rewrite H1. simpl. rewrite <- H1. rewrite H.  simpl in E1. rewrite E1. reflexivity.
+        ** simpl. reflexivity.
+        ** rewrite <- E4. simpl. rewrite H17. rewrite <- E4 in H19. simpl in H19. destruct (have_string "res1" M1) eqn:EE1. discriminate. reflexivity. 
+        ** rewrite <- E4. simpl. rewrite H18. rewrite <- E4 in H20. simpl in H20. destruct (have_string "res2" M1) eqn:EE1. discriminate. reflexivity. 
+        ** rewrite <- E4. eapply multi_step. apply beta_appabs. eapply multi_step. simpl. apply beta_l. apply subst_lemma1. apply H13. eapply multi_step.
+           apply beta_r. apply beta_l. apply subst_lemma1. rewrite <-E4 in H15. simpl in H15. destruct (have_string "s" M1). discriminate. reflexivity.
+           apply multib_eq_be. apply beta_symm. apply multib_eq_be. eapply multi_step. apply beta_r. apply beta_l. apply subst_lemma1. rewrite E4. apply E1.
+           apply multib_eq_be. apply beta_refl.
+     * eapply multi_step. apply multib_eq_be. apply IHM2. 
+        ** rewrite <- E4 in H0. simpl in H0. rewrite <- E4 in E1. rewrite E1 in H0. rewrite E2 in H0. rewrite E4 in H0. destruct H0. apply H21.
+        ** rewrite <- E4 in H5. simpl in H5. destruct (have_string "s1" M1) eqn:EE1. discriminate. apply H5.
+        ** rewrite <- E4 in H6. simpl in H6. destruct (have_string "s2" M1) eqn:EE1. discriminate. apply H6.
+        ** rewrite <- E4 in H15. simpl in H15. destruct (have_string "s" M1) eqn:EE1. discriminate. apply H15.
+        ** rewrite <- E4 in H19. simpl in H19. destruct (have_string "res1" M1) eqn:EE1. discriminate. apply H19. 
+        ** rewrite <- E4 in H20. simpl in H20. destruct (have_string "res2" M1) eqn:EE1. discriminate. apply H20.
+        ** rewrite <- E4 in E1. rewrite <- E4. simpl. apply eqb_eq in H1. rewrite H1. simpl. rewrite <- H1. rewrite H.  simpl in E1. rewrite E1. reflexivity.
+        ** simpl. reflexivity.
+        ** rewrite <- E4. simpl. rewrite H17. rewrite <- E4 in H19. simpl in H19. destruct (have_string "res1" M1) eqn:EE1. discriminate. reflexivity. 
+        ** rewrite <- E4. simpl. rewrite H18. rewrite <- E4 in H20. simpl in H20. destruct (have_string "res2" M1) eqn:EE1. discriminate. reflexivity. 
+        ** rewrite <- E4. eapply multi_step. apply beta_appabs. eapply multi_step. simpl. apply beta_l. apply subst_lemma1. apply H13. eapply multi_step.
+           apply beta_r. apply beta_l. apply subst_lemma1. rewrite <-E4 in H15. simpl in H15. destruct (have_string "s" M1). discriminate. reflexivity.
+           apply multib_eq_be. apply beta_symm. apply multib_eq_be. eapply multi_step. apply beta_r. apply beta_l. apply subst_lemma1. rewrite E4. apply E1.
+           apply multib_eq_be. apply beta_refl.
+      * eapply multi_step. apply multib_eq_be. apply IHM2. 
+        ** rewrite <- E4 in H0. simpl in H0. rewrite <- E4 in E1. rewrite E1 in H0. rewrite E2 in H0. rewrite E4 in H0. destruct H0. apply H21.
+        ** rewrite <- E4 in H5. simpl in H5. destruct (have_string "s1" M1) eqn:EE1. discriminate. apply H5.
+        ** rewrite <- E4 in H6. simpl in H6. destruct (have_string "s2" M1) eqn:EE1. discriminate. apply H6.
+        ** rewrite <- E4 in H15. simpl in H15. destruct (have_string "s" M1) eqn:EE1. discriminate. apply H15.
+        ** rewrite <- E4 in H19. simpl in H19. destruct (have_string "res1" M1) eqn:EE1. discriminate. apply H19. 
+        ** rewrite <- E4 in H20. simpl in H20. destruct (have_string "res2" M1) eqn:EE1. discriminate. apply H20.
+        ** rewrite <- E4 in E1. rewrite <- E4. simpl. apply eqb_eq in H1. rewrite H1. simpl. rewrite <- H1. rewrite H.  simpl in E1. rewrite E1. reflexivity.
+        ** simpl. reflexivity.
+        ** rewrite <- E4. simpl. rewrite H17. rewrite <- E4 in H19. simpl in H19. destruct (have_string "res1" M1) eqn:EE1. discriminate. reflexivity. 
+        ** rewrite <- E4. simpl. rewrite H18. rewrite <- E4 in H20. simpl in H20. destruct (have_string "res2" M1) eqn:EE1. discriminate. reflexivity. 
+        ** rewrite <- E4. eapply multi_step. apply beta_appabs. eapply multi_step. simpl. apply beta_l. apply subst_lemma1. apply H13. eapply multi_step.
+           apply beta_r. apply beta_l. apply subst_lemma1. rewrite <-E4 in H15. simpl in H15. destruct (have_string "s" M1). discriminate. reflexivity.
+           apply multib_eq_be. apply beta_symm. apply multib_eq_be. eapply multi_step. apply beta_r. apply beta_l. apply subst_lemma1. rewrite E4. apply E1.
+           apply multib_eq_be. apply beta_refl.
+     * eapply multi_step. apply multib_eq_be. apply IHM2. 
+        ** rewrite <- E4 in H0. simpl in H0. rewrite <- E4 in E1. rewrite E1 in H0. rewrite E2 in H0. rewrite E4 in H0. destruct H0. apply H21.
+        ** rewrite <- E4 in H5. simpl in H5. destruct (have_string "s1" M1) eqn:EE1. discriminate. apply H5.
+        ** rewrite <- E4 in H6. simpl in H6. destruct (have_string "s2" M1) eqn:EE1. discriminate. apply H6.
+        ** rewrite <- E4 in H15. simpl in H15. destruct (have_string "s" M1) eqn:EE1. discriminate. apply H15.
+        ** rewrite <- E4 in H19. simpl in H19. destruct (have_string "res1" M1) eqn:EE1. discriminate. apply H19. 
+        ** rewrite <- E4 in H20. simpl in H20. destruct (have_string "res2" M1) eqn:EE1. discriminate. apply H20.
+        ** rewrite <- E4 in E1. rewrite <- E4. simpl. apply eqb_eq in H1. rewrite H1. simpl. rewrite <- H1. rewrite H.  simpl in E1. rewrite E1. reflexivity.
+        ** simpl. reflexivity.
+        ** rewrite <- E4. simpl. rewrite H17. rewrite <- E4 in H19. simpl in H19. destruct (have_string "res1" M1) eqn:EE1. discriminate. reflexivity. 
+        ** rewrite <- E4. simpl. rewrite H18. rewrite <- E4 in H20. simpl in H20. destruct (have_string "res2" M1) eqn:EE1. discriminate. reflexivity. 
+        ** rewrite <- E4. eapply multi_step. apply beta_appabs. eapply multi_step. simpl. apply beta_l. apply subst_lemma1. apply H13. eapply multi_step.
+           apply beta_r. apply beta_l. apply subst_lemma1. rewrite <-E4 in H15. simpl in H15. destruct (have_string "s" M1). discriminate. reflexivity.
+           apply multib_eq_be. apply beta_symm. apply multib_eq_be. eapply multi_step. apply beta_r. apply beta_l. apply subst_lemma1. rewrite E4. apply E1.
+           apply multib_eq_be. apply beta_refl.
+    + eapply multi_step. simpl. rewrite E1. rewrite E2. apply subst_lemma1. simpl. rewrite H. rewrite E1. rewrite E2. reflexivity.
+       apply multib_eq_be. apply beta_symm. apply multib_eq_be. eapply multi_step. apply beta_r. apply subst_lemma1. simpl. rewrite E1. apply E2. apply multib_eq_be. apply beta_refl.
+  - simpl in H0. destruct (F =? s) eqn:E1.
+    + simpl. rewrite E1. eapply multi_step. apply subst_lemma1. simpl. rewrite H. rewrite E1. reflexivity. apply multib_eq_be. apply beta_refl.
+    + simpl. rewrite E1. destruct (have_string F M) eqn:E2. destruct H0. eapply multi_step. apply subst_lemma1. simpl. rewrite H. rewrite E1. apply E2. apply multib_eq_be. apply beta_symm. apply multib_eq_be.
+      eapply multi_step. apply beta_r. apply beta_abs. apply subst_lemma1. apply E2. apply multib_eq_be. apply beta_refl.
+  - simpl. eapply multi_step. apply beta_l. apply subst_lemma1. apply H. apply multib_eq_be. apply beta_refl.
+  - simpl. eapply multi_step. apply beta_l. apply subst_lemma1. apply H. apply multib_eq_be. apply beta_refl.
+  - simpl in H0. destruct (have_string F M1) eqn:E1. destruct H0. destruct (have_string F M2) eqn:E2. destruct H0. destruct (have_string F M3) eqn:E3. destruct H0.
+    apply multib_eq_be. apply beta_symm. apply multib_eq_be. eapply multi_step. apply beta_r. apply subst_lemma1. simpl. rewrite E1. rewrite E2. rewrite E3. reflexivity.
+    simpl. rewrite E1. rewrite E2. rewrite E3. apply multib_eq_be. apply beta_symm. apply multib_eq_be. eapply multi_step. apply subst_lemma1.  simpl. rewrite E1. rewrite E2. rewrite E3. rewrite H. reflexivity.
+    apply multib_eq_be. apply beta_refl.
+  - simpl in H0. destruct(F =? s) eqn:E0; destruct(have_string F M1) eqn:E1. destruct H0. 
+    + simpl. rewrite E0. rewrite E1. eapply multi_step. apply subst_lemma1. simpl. rewrite H. rewrite E0. apply E1. apply multib_eq_be. apply beta_symm. apply multib_eq_be. eapply multi_step.
+      apply beta_r. apply beta_let1. apply subst_lemma1. apply E1. apply beta_refl. apply multib_eq_be. apply beta_refl.
+    + destruct H0. 
+    + destruct(have_string F M2) eqn:E2. destruct H0. eapply multi_step. simpl. apply subst_lemma1. simpl. rewrite E0. rewrite E1. rewrite E2. simpl. rewrite H. rewrite E0. rewrite E1. rewrite E2. reflexivity.
+      rewrite E0. rewrite E1. rewrite E2. 
+      apply multib_eq_be. apply beta_symm. apply multib_eq_be. eapply multi_step. apply beta_r. apply subst_lemma1. simpl. rewrite E0. rewrite E1. rewrite E2. reflexivity.
+      apply multib_eq_be. apply beta_refl.
+  - simpl in H0. destruct(have_string F M) eqn:E1. destruct H0. eapply multi_step. simpl. rewrite E1. apply subst_lemma1. simpl. rewrite H. apply E1.
+    apply multib_eq_be. apply beta_symm. apply multib_eq_be. eapply multi_step. apply beta_r. apply subst_lemma1. simpl. apply E1.
+    apply multib_eq_be. apply beta_refl.
+  Qed.
+
+(* Theorem m_k : forall (F k:tm)(n: nat),
   halt k->
   is_recursion F->
   app k (app F n) =b app (app (trans_to_tail_recursion F) n) k.
@@ -722,9 +1247,9 @@ Proof.
                         +++ simpl. eapply multi_step. 
                           ++++ apply beta_r. apply subst_lemma2. apply subst_lemma2. apply subst_lemma1. apply E8.
                           ++++ rewrite gen_lemma2.   
-            
+             *)
 
-Theorem m_k__k_m : forall (F k M:tm) (f:string),
+(*  Theorem m_k__k_m : forall (F k M:tm) (f:string),
   is_fix_string F f->
   is_recursion F -> 
   trans_M f k M =b app k M.
@@ -736,23 +1261,9 @@ Proof.
 
   unfold is_recursion in H0.
   destruct t1 eqn:E4; try destruct H0.
-  destruct t2 eqn:E5; try destruct H0.
+  destruct t2 eqn:E5; try destruct H0. *)
   
 
-Lemma be_tttr2 : forall (k M:tm) ,
-  M =b trans_to_tail_recursion M
-.
-Proof. Admitted.
-Lemma be_tttr : forall (k M:tm) ,
-  trans_M k M =b app k M
-.
-Proof.
-  intros.
-  induction M; try apply beta_refl.
-  simpl.   
-    
-  
-Admitted.
   
 
 
@@ -764,7 +1275,7 @@ Compute trans_to_tail_recursion fact.
 
 
 Example test_mlt_cont_trans1 :
-  multistep (app (app (trans_to_tail_recursion fact) 4) (abs "s" Nat "s")) 24.
+  multistep (app (app (trans_to_tail_recursion fact) 4) (abs "s" "s")) 24.
 Proof.
   unfold trans_to_tail_recursion.
   unfold fact.
@@ -773,7 +1284,7 @@ Proof.
   Qed.
 
 Example test_mlt_cont_trans2 :
-  multistep (app (app (trans_to_tail_recursion fact2) 4)(abs "s" Nat "s"))  24.
+  multistep (app (app (trans_to_tail_recursion fact2) 4)(abs "s" "s"))  24.
 Proof.
   unfold trans_to_tail_recursion.
   unfold fact2.
@@ -784,7 +1295,7 @@ Proof.
 Compute trans_to_tail_recursion fact_pls.
 
 Example test_mlt_pls_cont_trans1 :
-  multistep (app (app (trans_to_tail_recursion fact_pls) 4) (abs "s" Nat "s")) 88.
+  multistep (app (app (trans_to_tail_recursion fact_pls) 4) (abs "s" "s")) 88.
 Proof.
   unfold trans_to_tail_recursion.
   unfold fact_pls.
@@ -809,8 +1320,8 @@ Proof.
 
 Definition double_recursion_fact :=
   tfix
-    (abs f (Arrow Nat Nat)
-      (abs x Nat
+    (abs f 
+      (abs x 
         (test0
            x
            1
@@ -827,7 +1338,7 @@ Definition double_fact_cont :=
   trans_to_tail_recursion double_recursion_fact.
 
 Example test_double_fact_cont:
-  multistep (app (app double_fact_cont 3)(abs "s" Nat "s")) 144.
+  multistep (app (app double_fact_cont 3)(abs "s" "s")) 144.
 Proof.
   unfold double_fact_cont.
   unfold trans_to_tail_recursion.
